theories/SLFMore.v
@@ -1,0 +1,789 @@
+
+Parameter example_trm_red : forall m,
+  red m (trm_app example_trm' (val_bool false)) m (val_int 1).
+
+
+
+Definition assertion := state -> Prop.
+Definition Hoare_triple (H:assertion) (t:trm) (Q:val->assertion) : Prop :=
+  forall h, H h ->
+  exists v h', red h t h' v /\ Q v h'.
+Parameter val_div : prim.
+
+
+
+(** * Hprop: Heap Predicates *)
+
+(** ** Definition of Separation Logic triples *)
+
+(** We will give a definition of the separating conjunction operator (star)
+    shortly afterwards. For the moment, let us assume a definition of [star]
+    to exist, and let us exploit it to define the semantics of a SL triple. *)
+
+Parameter star : assertion -> assertion -> assertion.
+
+Notation "H1 '\*' H2" := (star H1 H2)
+  (at level 41, right associativity).
+
+(** Recall the definition of Separation Logic triples from the introduction.
+
+[[
+  Definition SL_triple (H:assertion) (t:trm) (Q:assertion) :=
+    forall (H':assertion), Hoare_triple (H \* H') t (Q \* H').
+]]
+
+    To adapt it to a language where terms output values, we need to
+    define what it means to compute the star of a postcondition [Q] of
+    type [val->assertion] and of an assertion [H].
+
+    To that end, we let [Q \*+ H'] denote [fun x => (Q x \* H')].
+    This postcondition characterizes the same output value as [Q],
+    but in an output heap extended with [H'].
+*)
+
+Notation "Q \*+ H" := (fun x => (Q x) \* H)
+  (at level 40).
+
+(** Using this piece of notation, the definition of triples from the
+    introduction is easily adapted. *)
+
+Definition triple_1 (H:assertion) (t:trm) (Q:val->assertion) :=
+  forall (H':assertion), Hoare_triple (H \* H') t (Q \*+ H').
+
+(** The definition above defines SL triples in terms of Hoare triples.
+    While this indirect definition is helpful for providing intuition,
+    a direct definition is better suited for conducting proofs.
+    If we unfold the intermediate definition of Hoare triples and
+    perform minor simplification, we obtain the definition shown below. *)
+
+Definition triple_2 (H:assertion) (t:trm) (Q:val->assertion) : Prop :=
+  forall H' h, (H \* H') h ->
+  exists v h', red h t h' v /\ (Q v \* H') h'.
+
+(** This definition reads as follows: for any input heap [h], and any
+    heap predicate [H'] describing the part of the heap not covered
+    by the precondition [H], there exists an output value [v] and an
+    output heap [h'] to which the term [t] evaluates starting from the
+    input heap [h], and such that a subset of the final heap is described
+    by the postcondition [Q] applied to the value [v], while the remaining
+    subset of the output heap corresponds is described by [H']. *)
+
+(** ** Slight change in terminology *)
+
+(** In Separation Logic, we usually manipulate only pieces of states,
+    as opposed to complete state. It is convenient to keep track of
+    the intention by using two distinct types:
+    - [state] denotes a complete state,
+    - [heap] denotes a piece of state.
+
+
+    In our formalism, both [state] and [heap] are represented as
+    finite maps from locations to values, so the distinction might
+    appear a bit artificial. Nevertheless, this distinction proves
+    very useful when extending Separation Logic with additional features,
+    such as "time credits" or "read-only permissions".
+    Thus, we introduce the following alias. *)
+
+Definition heap : Type := state. (* intended to represent a piece of state *)
+
+(** In practice, we use type [state] when defining the evaluation rules,
+    and we use the type [heap] to denote the argument of an assertion.
+    In the rare cases where an entity is used at the same time in an
+    evaluation rule and as argument of an assertion, we use type [heap]. *)
+
+(** A Separation Logic assertion is a predicate over a piece of state.
+    Thus, it has type [heap -> Prop]. The type of such _heap predicates_
+    is written [hprop]. *)
+
+Definition hprop := heap -> Prop.
+
+(** With the new terminology, and with placing the term [t] as first
+    argument, the definition of SL triples becomes: *)
+
+Definition triple_3 (t:trm) (H:hprop) (Q:val->hprop) : Prop :=
+  forall H' h, (H \* H') h ->
+  exists v h', red h t h' v /\ (Q v \* H') h'.
+
+Notation "'triple'" := triple_3.
+
+(** By convention, we let [H] range over heap predicates (of type [hprop]),
+    and [Q] range over postconditions (of type [val->hprop]). *)
+
+
+(** * Fundamental heap predicates *)
+
+(** We next present the definitions of the fundamental building blocks for
+    constructing heap predicates. These building blocks are:
+
+    - [\[]] denotes the empty heap predicate.
+    - [\[P]] denotes the empty heap predicate and asserts that [P] is true.
+    - [l ~~> v] describes a single memory cell, at location [l], with
+      contents [v].
+    - [H1 \* H2] denotes the separating conjunction of two heap predicates.
+    - [\exists x, H] denotes an existential quantification at the level of
+      heap predicates.
+
+    As we will see through this section, each of these heap predicates is
+    defined as a function of the form [fun (h:heap) -> (...:Prop)].
+
+    What makes Separation Logic works so smoothly in practice is that
+    the aforementioned fundamental heap predicates are the only ones that are
+    defined directly as functions from heap to propositions. All user-defined
+    heap predicates are then defined as combination of these fundamental
+    heap predicates. It is thus essential to have a deep understanding of
+    the meaning of the fundamental heap predicates. *)
+
+(* SLIDE: grammar-of-basic-heap-predicates *)
+
+(** ** Points-to predicate *)
+
+(** The points-to heap predicate is written [l ~~> v], which is a notation for
+    [hsingle l v]. This heap predicate characterizes a heap [h] that is made
+    of a single memory cell, at location [l], with contents [v]. In addition,
+    [hsingle l v] captures the property that [l] is not the [null] location.
+    The formal definition is as follows: *)
+
+Definition hsingle (l:loc) (v:val) : hprop :=
+  fun h => h = fmap_single l v /\ l <> null.
+
+Notation "l '~~>' v" := (hsingle l v)
+  (at level 32, no associativity).
+
+(** For example, the following specification of [incr r] indicates
+    that it executes safely assuming that location [r] is allocated
+    with contents [2], and that it updates this location to contain [3].
+    The evaluation of [incr r] returns some value [v], which as we will
+    see soon afterwards, may be specified to be the unit value. *)
+
+Parameter (incr:val) (r:loc).
+
+Parameter hsingle_demo :
+  triple (incr r)
+    (r ~~> 2) (* precondition *)
+    (fun v => r ~~> 3). (* postcondition *)
+
+(** The general specification of the [incr] function involves a universal
+    quantification over the initial contents of the cell, as shown below. *)
+
+Parameter triple_incr : forall (n:int),
+  triple (incr r)
+    (r ~~> n)
+    (fun v => r ~~> (n+1)).
+
+(* EX1! (triple_augment) *)
+(** State a specification for the term [val_augment r m], which takes
+    as arguments a location [r] and an integer [m], and updates the cell
+    at location [r] by adding [m] to its original contents. *)
+
+Parameter val_augment : val.
+
+(* SOLUTION *)
+Parameter triple_augment : forall (r:loc) (n m:int),
+  triple (val_augment r m)
+    (r ~~> n)
+    (fun v => r ~~> (n + m)).
+(* /SOLUTION *)
+
+(** [] *)
+
+
+(** ** Star predicate *)
+
+(** The star predicate is written [H1 \* H2], which is a notation for
+    [hstar H1 H2]. This heap predicate characterizes a heap [h] that
+    is composed of two disjoint parts, call them [h1] and [h2], such that
+    the first one satisfies [H1] and the second one satisfies [H2].
+    Together, the propositions [state_disjoint h1 h2] and [h = state_union h1 h2]
+    assert that [h1] and [h2] really constitute a partition of [h] in two
+    disjoint parts. *)
+
+Definition hstar (H1 H2:hprop) : hprop :=
+  fun h => exists (h1 h2:heap),
+       H1 h1
+    /\ H2 h2
+    /\ fmap_disjoint h1 h2
+    /\ h = fmap_union h1 h2.
+
+Notation "H1 '\*' H2" := (hstar H1 H2)
+  (at level 41, right associativity).
+
+(** Consider for example the following specification of [incr r] which captures
+    the fact that it does not modify the contents of another reference [s]. *)
+
+Parameter hstar_demo : forall (s:loc) (n m:int),
+  triple (incr r)
+    (r ~~> n \* s ~~> m)
+    (fun v => r ~~> (n+1) \* s ~~> m).
+
+(* EX2! (triple_swap) *)
+(** State a specification for the term [val_swap r s], which takes as argument
+    two distinct locations [r] and [s], with respective contents two integers [n]
+    and [m], and that swaps the contents of the two locations. *)
+
+Parameter val_swap : val.
+
+(* SOLUTION *)
+Parameter triple_swap : forall (r s:loc) (n m:int),
+  triple (val_swap r s)
+    (r ~~> n \* s ~~> m)
+    (fun v => r ~~> m \* s ~~> n).
+(* /SOLUTION *)
+
+(** [] *)
+
+(* EX1! (hstar_comm) *)
+(** Prove that separating conjunction is commutative, in the sense that any
+    heap satisfying [H1 \* H2] also satisfies [H2 \* H1]. The proof involves
+    the two following results on finite maps: symmetry of the disjointness
+    predicate, and commutativity of the union of disjoint heaps. *)
+
+Parameter fmap_disjoint_sym : forall (h1 h2:heap),
+  fmap_disjoint h1 h2 ->
+  fmap_disjoint h2 h1.
+
+Parameter fmap_union_comm_of_disjoint : forall (h1 h2:heap),
+  fmap_disjoint h1 h2 ->
+  fmap_union h1 h2 = fmap_union h2 h1.
+
+Lemma hstar_comm : forall (H1 H2:hprop) (h:heap),
+  ((H1 \* H2) h) ->
+  ((H2 \* H1) h).
+Proof.
+  (* ADMITTED *)
+  introv (h1&h2&P1&P2&D&E). exists h2 h1. splits.
+  { apply P2. }
+  { apply P1. }
+  { apply fmap_disjoint_sym. auto. }
+  { rewrite fmap_union_comm_of_disjoint. auto. auto. }
+Qed.
+  (* /ADMITTED *)
+
+(** [] *)
+
+(** An essential property of Separation Logic is that it is never possible
+    to construct a heap satisfying a heap predicate of the form
+    [(r ~~> ..) \* (r ~~> ..)]. Indeed, there is no way to exhibit two
+    disjoint heaps that both have [r] in their domain. *)
+
+Lemma hstar_hsingle_same_loc_inv : forall (l:loc) (v1 v2:val) (h:heap),
+  ((l ~~> v1) \* (l ~~> v2)) h ->
+  False.
+Proof.
+  introv (h1&h2&P1&P2&D&E). destruct P1 as (E1&N1). destruct P2 as (E2&N2).
+  subst. applys* fmap_disjoint_single_single_same_inv.
+Qed.
+
+(** Now that the separating conjunction is properly defined,
+    we update the definition of [triple] to use that definition,
+    instead of the abstract [star] operator that assumed previously. *)
+
+Definition triple_4 (t:trm) (H:hprop) (Q:val->hprop) : Prop :=
+  forall H' h, (H \* H') h ->
+  exists v h', red h t h' v /\ (Q v \* H') h'.
+
+(** Thereafter, [triple] is a shorthand for [triple_4]. *)
+
+Notation "'triple'" := triple_4.
+
+(* QUIZ *)
+(** Is the following triple true or false? *)
+Parameter triple_cell_twice : forall (r:loc) (n:int),
+  triple (val_unit)
+    (r ~~> n \* r ~~> n)
+    (fun v => r ~~> (n+1) \* r ~~> (n+1)).
+(* INSTRUCTORS: The triple is true because its precondition is equivalent
+   to false, i.e. it cannot be satisfied by any input heap. *)
+(* /QUIZ *)
+
+(* EX2! (triple_cell_twice) *)
+(** Prove the above lemma.
+    Hint: unfold the definition of [triple], a.k.a. [triple_4],
+    and decompose the assumption on the input heap in order to
+    derive a contradiction using lemma [hstar_hsingle_same_loc_inv]. *)
+
+Lemma triple_cell_twice' : forall (r:loc) (n:int),
+  triple (val_unit)
+    (r ~~> n \* r ~~> n)
+    (fun v => r ~~> (n+1) \* r ~~> (n+1)).
+Proof.
+  (* ADMITTED *)
+  intros. unfold triple_4. intros H' h M. destruct M as (h1&h2&P1&P2&D&E).
+  false. eapply hstar_hsingle_same_loc_inv. apply P1.
+Qed.
+  (* /ADMITTED *)
+
+(** [] *)
+
+
+(** ** Pure heap predicate *)
+
+(** The _empty heap predicate_ is written [ \[] ], which is a notation for
+    [hempty]. It characterizes exactly heaps that are empty. *)
+
+Definition hempty : hprop :=
+  fun h => h = fmap_empty.
+
+Notation "\[]" := (hempty)
+  (at level 0).
+
+(** The _pure heap predicate_ extends the empty heap predicate by capturing
+    not just the fact that its argument is the heap is empty, but also that
+    some proposition [P] is true. The pure heap predicate is written [ \[P] ],
+    which is a notation for [hpure P]. It is defined as follows: *)
+
+Definition hpure (P:Prop) : hprop :=
+  fun h => (h = fmap_empty /\ P).
+
+Notation "\[ P ]" := (hpure P)
+  (at level 0, P at level 99, format "\[ P ]").
+
+(** The empty heap predicate and the pure heap predicate are systematically
+    involved in the precondition and the postcondition of pure functions, i.e.
+    functions that do not involve side effects. Consider for example the
+    specification of the successor function. The precondition assumes
+    an empty input heap. The postcondition asserts an empty input heap, and
+    moreover asserts that the output value is one unit greater than the
+    input argument. *)
+
+Parameter triple_succ : forall (n:int),
+  triple (val_add (val_int n))
+    \[]
+    (fun (r:val) => \[r = val_int (n + 1)]).
+
+(** Observe by executing [Print triple_succ] that the [val_int] constructor
+    is in fact not displayed by Coq. Indeed, it is declared as a coercion.
+    In fact, we do not need to write [val_int] in the triple, as Coq is
+    able to infer its occurences. Thus, we may write more concisely: *)
+
+Parameter triple_succ' : forall (n:int),
+  triple (val_add n)
+    \[]
+    (fun (r:val) => \[r = n + 1]).
+
+(** As another example, consider the specification of the addition primitive
+    function. The precondition assumes an empty input heap. The postcondition
+    asserts an empty input heap, and moreover asserts that the output value
+    is the sum of the two arguments. *)
+
+Parameter triple_add : forall (n1 n2:int),
+  triple (val_add n1 n2)
+    \[]
+    (fun (r:val) => \[r = n1 + n2]).
+
+(** Note that the specification tells nothing about the behavior of
+    addition in the case where the two arguments are not both integer values. *)
+
+(** Symmetrically to its use in postconditions, the pure heap predicate may
+    appear in preconditions to describe requirements on the arguments.
+    For example, division expects a nonzero integer as second argument. *)
+
+Parameter triple_div : forall (n1 n2:int),
+  triple (val_div n1 n2)
+    \[n2 <> 0]
+    (fun (r:val) => \[r = n1 + n2]).
+
+(** While the above formulation is perfectly valid, it is more convenient in
+    practice to follow an alternative, logically equivalent presentation,
+    whereby the pure preconditions appear as Coq hypotheses outside the triple.
+    In the case of the division, this alternative presentation amounts to
+    asserting [n2 <> 0] as hypothesis prior to the triple: *)
+
+Parameter triple_div' : forall (n1 n2:int),
+  n2 <> 0 ->
+  triple (val_div n1 n2)
+    \[]
+    (fun (r:val) => \[r = n1 + n2]).
+
+(** Throughout the course, we will follow the convention that pure preconditions
+    appear as hypotheses prior to the triple. Thus, preconditions will only
+    be used to describe the shape of the heap. *)
+
+(** DEPRECATED !!
+
+    The pure heap predicate is useful not just for specifying pure functions,
+    but also for specifying effectful functions, to assert properties about
+    the output value or the output heap. For example, in the specification
+    of [incr r] shown below, the pure heap predicate [ \[v = val_unit] ] asserts
+    that the evaluation of [incr r] returns the unit value. This heap predicate
+    comes in addition to the points-to heap predicate that describes the output
+    heap. *)
+
+Parameter hpure_demo :
+  triple (incr r)
+    (r ~~> 2)
+    (fun v => (r ~~> 3)).
+
+(** Above, observe that the two heap predicates from the postcondition
+    are separated by the star operator. This operator asserts that the output
+    heap decomposes into two disjoint parts: an empty heap, which satisfies
+    the predicate [ \[v = val_unit] ], and a singleton heap, which satisfies
+    the assertion [r ~~> 3]. Such use of the separating conjunction, where one
+    part corresponds to the empty heap, may appear somewhat unexpected at
+    first, but it is perfectly well-defined and corresponds to a specification
+    pattern that we will see over and over again.
+
+    As another example, consider the specification below for the primitive
+    [val_get], used to read in a memory cell. Assuming the argument [l] to
+    correspond to a location at which some value [v] is stored, the read
+    operation executes safely and returns an output value, call it [x],
+    which is such that [x = v]. The piece of heap, described by [l ~~> v],
+    is returned unchanged in the postcondition. *)
+
+Parameter triple_get : forall (v:val) (l:loc),
+  triple (val_get l)
+    (l ~~> v)
+    (fun (r:val) => \[r = v] \* (l ~~> v)).
+
+(** Remark: above, [val_get l] is interpreted using coercions, and stands for
+    [trm_app (trm_val (val_prim val_get)) (trm_val (val_loc l))]. *)
+
+(* EX2! (triple_set) *)
+(** State a specification for the term [val_set l v], which updates the
+    location [l] with the value [v]. Make sure to specify that the update
+    operation returns the unit value. *)
+
+(* SOLUTION *)
+Parameter triple_set : forall (v w:val) (l:loc),
+  triple (val_set l v)
+    (l ~~> w)
+    (fun (r:val) => l ~~> v).
+(* /SOLUTION *)
+
+(** [] *)
+
+(* EX2! (triple_free) *)
+(** State a specification for the term [val_free l], which assumes a
+    location [l] to be allocated, and explicitly disposes this location.
+    Note that such a free operation usually does not appear in programming
+    languages featuring a GC, but is commonplace in other languages.
+    The postcondition should  assert that the return value is unit, and
+    not mention the location [l] anymore, effectively banning any subsequent
+    access to this location. *)
+
+Parameter val_free : val.
+
+(* SOLUTION *)
+Parameter triple_free : forall (v:val) (l:loc),
+  triple (val_free l)
+    (l ~~> v)
+    (fun (r:val) => \[r = val_unit]).
+(* /SOLUTION *)
+
+(** [] *)
+
+(* EX1? (hpure_true_iff_hempty) *)
+(** Prove that a heap satisfies the heap predicate [\[True]] if and only
+    if it satisfies the empty heap predicate. *)
+
+Lemma hpure_true_iff_hempty : forall (h:heap),
+  (\[True] h) <-> (\[] h).
+Proof.
+  (* ADMITTED *)
+  intros. split.
+  { intros (M&N). hnf. auto. }
+  { intros M. split. { hnf in M. auto. } { auto. } }
+Qed.
+  (* /ADMITTED *)
+
+(** [] *)
+
+(** The next lemma establishes that the heap predicate [H \* \[]]
+    is equivalent to [H]. Its proof relies on two handy tactics,
+    that will be useful for proving numerous metatheory results.
+    - The tactic [fmap_eq] proves equality between finite maps,
+      e.g. [fmap_union h fmap_empty = h].
+    - The tactic [fmap_disjoint] proves obvious disjointness results,
+      e.g. [fmap_disjoint h fmap_empty], or [fmap_disjoint h1 h2]
+      when [fmap_disjoint h2 h1] appears in the context.
+
+    The proof is as follows. *)
+
+Lemma hstar_hempty_iff : forall (H:hprop) (h:heap),
+  ((H \* \[]) h) <-> (H h).
+Proof.
+  intros. split.
+  { intros (h1&h2&P1&P2&D&E). hnf in P2. subst. fmap_eq. auto. }
+  { intros M. exists h (fmap_empty:heap). splits.
+    { auto. }
+    { hnf. auto. }
+    { fmap_disjoint. }
+    { fmap_eq. } }
+Qed.
+
+(** Observe that we need to provide an explicit type annotation in
+    [(fmap_empty:heap)], because [fmap_empty] is a polymorphic
+    constructor, and the "exists" tactic is too limited to figure out
+    by itself the required types from the current proof obligation. *)
+
+(* EX2? (hstar_hpure_iff) *)
+(** Establish a generalization of the above lemma, proving that the heap
+    predicate [H \* \[P]] is equivalent to [H] when proposition [P] holds. *)
+
+Lemma hstar_hpure_iff : forall (H:hprop) (P:Prop) (h:heap),
+  ((H \* \[P]) h) <-> ((H h) /\ P).
+Proof.
+  (* ADMITTED *)
+  intros. split.
+  { intros (h1&h2&P1&(P2&P2')&D&E). subst. fmap_eq. auto. }
+  { intros (M&N). exists h (fmap_empty:heap). splits.
+    { auto. }
+    { hnf. auto. }
+    { fmap_disjoint. }
+    { fmap_eq. } }
+Qed.
+  (* /ADMITTED *)
+
+(** [] *)
+
+
+(** ** Existential heap predicate *)
+
+(** The _existential heap predicate_ provides existential quantification
+    at the level of heap predicates. It is written [\exists x, H], which
+    is a notation for [hexists (fun x => H)]. It is the counterpart of the
+    normal existential quantification on propositions, which is written
+    [exists x, P], a notation for [ex (fun x => P)].
+
+    The Coq definition of [hexists] is polymorphic in the type of [x].
+    The type of [x] is called [A] below. The argument of [hexists], called [J]
+    below, is typically of the form [fun x => H]. It has type [A->hprop]. *)
+
+Definition hexists (A:Type) (J:A->hprop) : hprop :=
+  fun h => exists x, J x h.
+
+Notation "'\exists' x1 , H" := (hexists (fun x1 => H))
+  (at level 39, x1 ident, H at level 50).
+
+(** The notation [\exists x1 x2 x3, H] shows useful to quantify several
+    arguments at once. *)
+
+Notation "'\exists' x1 x2 , H" := (\exists x1, \exists x2, H)
+  (at level 39, x1 ident, x2 ident, H at level 50).
+Notation "'\exists' x1 x2 x3 , H" := (\exists x1, \exists x2, \exists x3, H)
+  (at level 39, x1 ident, x2 ident, x3 ident, H at level 50).
+(** The notation [\exists (x:T), H] allows us to provide an explicit
+    type annotation. *)
+
+Notation "'\exists' ( x1 : T1 ) , H" := (hexists (fun x1:T1 => H))
+  (at level 39, x1 ident, H at level 50, only parsing).
+
+Notation "'\exists' ( '_' : T1 ) , H" := (hexists (fun _:T1 => H))
+  (at level 39, H at level 50). (* useful when quantifying over proof terms *)
+
+(** The main role of existential quantification is to introduce abstraction.
+    For example, assume that we want to specify the increment function
+    by saying that it updates the contents of its target location to
+    some greater contents, without revealing that the new contents is exactly
+    one unit greater. Then, for a precondition [r ~~> n], we would consider
+    the postcondition [\exists m, (r ~~> m) \* \[m > n]]. *)
+
+Parameter hexists_demo : forall (n:int),
+  triple (incr r)
+    (r ~~> n)
+    (fun v => \[v = val_unit] \* \exists (m:int), (r ~~> m) \* \[m > n]).
+
+(** Existential quantification is also useful to specify output values
+    when they have a specific shape. For example, consider the operation
+    called [val_ref], which allocates and initializes one memory cell
+    with some contents [v]. A call to [val_ref] executes safely in the
+    empty heap. The output value of its evaluation is a value, call it [r],
+    which is of the form [val_loc l] for _some_ location [l]. The output
+    heap satisfies [l ~~> v] for that particular [l]. As shown below, the
+    location [l] gets existentially quantified in the postcondition. *)
+
+Parameter triple_ref : forall (v:val),
+  triple (val_ref v)
+    \[]
+    (fun (r:val) => \exists (l:loc), \[r = val_loc l] \* (l ~~> v)).
+
+(* EX2! (triple_ref_of_ref) *)
+(** Consider the term [val_ref (val_ref 3)], which allocates a memory
+    cell with contents [3], at some location [l], then allocates a
+    another memory cell with contents [l], at some location [l'], and
+    finally returns the location [l']. State a specification for that
+    term. *)
+
+(* SOLUTION *)
+Parameter triple_ref_of_ref :
+  triple (val_ref (val_ref 3))
+    \[]
+    (fun (r:val) =>
+        \exists (l:loc), \[r = val_loc l] \* \exists (l':loc),
+                         (l ~~> l') \* (l' ~~> 3)).
+(* /SOLUTION *)
+
+(** [] *)
+
+(* EX1? (hexists_permut) *)
+(** Prove that [\exists x, \exists y, K x y] is equivalent to
+    [\exists y, \exists x, K x y]. *)
+
+Lemma hexists_permut : forall (A B:Type) (K:A->B->hprop) (h:heap),
+  ((\exists x, \exists y, K x y) h) ->
+  ((\exists y, \exists x, K x y) h).
+Proof.
+  (* ADMITTED *)
+  introv (x&y&M). exists y x. apply M.
+Qed.
+  (* /ADMITTED *)
+
+(** [] *)
+
+(* EX2? (hpure_iff_hexists_prop) *)
+(** Prove that a heap satisfies the heap predicate [\[P]] for some
+    proposition [P] if and only if it satisfies the heap predicate
+    [\exists (p:P), \[]]. The latter describes a empty heap and
+    asserts the existence of a proof term [p] of type [P]. In Coq,
+    asserting the existence of such a proof term of type [P] is
+    equivalent to asserting that [P] is a true proposition. *)
+
+Lemma hpure_iff_hexists_proof : forall (P:Prop) (h:heap),
+  (\[P] h) <-> ((\exists (p:P), \[]) h).
+Proof.
+  (* ADMITTED *)
+  intros. split.
+  { intros (M&p). exists p. hnf. auto. }
+  { intros (p&M). hnf in M. split. { auto. } { auto. } }
+Qed.
+  (* /ADMITTED *)
+
+(** [] *)
+
+
+(** ** Summary *)
+
+(** The fundamental heap predicates are written:
+    - [\[]]
+    - [\[P]]
+    - [l ~~> v]
+    - [H1 \* H2]
+    - [\exists x, H].
+
+    and they are defined as follows. *)
+
+(* SLIDE: definition-of-basic-heap-predicates *)
+
+Module Type Fundamental.
+
+Definition hempty : hprop :=
+  fun h => h = fmap_empty.
+
+Definition hpure (P:Prop) : hprop :=
+  fun h => h = fmap_empty /\ P.
+
+Definition hsingle (l:loc) (v:val) : hprop :=
+  fun h => h = fmap_single l v /\ l <> null.
+
+Definition hstar (H1 H2:hprop) : hprop :=
+  fun h => exists h1 h2,
+       H1 h1
+    /\ H2 h2
+    /\ fmap_disjoint h1 h2
+    /\ h = fmap_union h1 h2.
+
+Definition hexists (A:Type) (J:A->hprop) : hprop :=
+  fun h => exists x, J x h.
+
+End Fundamental.
+
+
+
+(** * Triples adapted for languages with garbage collection *)
+
+(** ** Motivating example *)
+
+(** Consider the program [Let x := val_ref 3 in 5], abbreviated below
+    as [t]. This program allocates a memory cell with contents [3], at some
+    location [x], and then returns [5]. In this program, the address
+    of the allocated memory cell is not returned, so it cannot be
+    subsequently accessed. Thus, one may argue that a natural specification
+    for this program is the same as that of a program that simply returns
+    the value [5], that is: *)
+
+Parameter t : trm. (* := [Let x := val_ref 3 in 5]. *)
+
+Parameter htop_example_1 :
+  triple t
+    \[]
+    (fun (r:val) => \[r = 5]).
+
+(** However, it turns out that the above triple cannot be derived with
+    respect to the definition of triples that we have considered so far.
+    The reason is simple: the memory cell that is allocated by the term
+    belongs to the heap structure, thus it must be described in the
+    postcondition. As a result, with the current definition, only the
+    following triple may be established: *)
+
+Parameter htop_example_2 :
+  triple t
+    \[]
+    (fun (r:val) => \[r = 5] \* \exists l, l ~~> 3).
+
+(** The remaining of this chapter describes a simple patch to the
+    definition of triple that would allow establishing the first
+    specification, which is much more natural. In short, we introduce
+    a mechanism that allows to discard any desired piece of state
+    from the postcondition. *)
+
+(** ** Patching triples using the top predicate *)
+
+(** To allow discarding any desired piece of state, we introduce a handy
+    heap predicate called "top", which is a predicate that holds of any
+    heap. This predicate is written [\Top], and defined as follows. *)
+
+Definition htop : hprop :=
+  fun (h:heap) => True.
+
+Notation "\Top" := (htop).
+
+(** In the definition of triples, we modify the specification of the
+    output heap from [(Q v \* H') h'] to [(Q v \* \Top \* H') h'].
+    Adding a [\Top] component effectively allows to _not describe_
+    in the postcondition pieces of state that have been allocated
+    during the execution of the term. *)
+
+Definition triple_5 (H:hprop) (t:trm) (Q:val->hprop) : Prop :=
+  forall H' h, (H \* H') h ->
+  exists v h', red h t h' v /\ (Q v \* \Top \* H') h'.
+
+(** Throughout the remaining of this course, the definition of
+    the predicate [triple] corresponds to the above definition.
+    It is defined in file [LambdaSep.v]. *)
+
+(* EX2! (htop_hstar_htop) *)
+(** Prove that [\Top \* \Top] is equivalent to [\Top], i.e., that
+    [\Top] is idempotent. Tactics [fmap_disjoint] and [fmap_eq]
+    are useful to complete the proof. *)
+
+Lemma htop_hstar_htop : forall (h:heap),
+  ((\Top \* \Top) h) <-> (\Top h).
+Proof.
+  (* ADMITTED *)
+  intros. split.
+  { intros (h1&h2&P1&P2&D&E). hnf. auto. }
+  { intros M. exists h (fmap_empty:heap). splits.
+    { hnf. auto. }
+    { hnf. auto. }
+    { fmap_disjoint. }
+    { fmap_eq. } }
+Qed.
+  (* /ADMITTED *)
+
+(** [] *)
+
+(* EX2? (htop_iff_hexists_heap) *)
+(** Prove that a heap satisfies the heap predicate [\[Top]] if and
+    only if it satisfies the predicate [\exists (H:hprop), H]. *)
+
+Lemma htop_iff_hexists_hprop : forall (P:Prop) (h:heap),
+  (\Top h) <-> (\exists H, H) h.
+Proof.
+  (* ADMITTED *)
+  intros. split.
+  { intros M. exists (= h). auto. }
+  { intros (H&M). hnf. auto. }
+Qed.
+  (* /ADMITTED *)
+
+(** [] *)
+
